examples/malloc.v
@@ -1,18 +1,39 @@
-From OLCoq Require Import syntax ol metatheory util set.
+From OLCoq Require Import assertion metatheory ol rules semantics set syntax theorems util.
 
-Definition buggy_program (x : nat) : cl :=
-  x <- malloc ⨟
-  [ var x ] <- 1
+(* Program with a potential null dereference memory error *)
+Example program x :=
+      x <- malloc ⨟
+      [ var x ] <- 1
 .
 
-Theorem spec x : ⊢ ⟨ ok ⟩ buggy_program x ⟨ var x --> 1 ⊕ Err ⟩.
+(* Proof using outcome logic that the program may have a
+   null dereference memory error *)
+Example has_potential_memory_error x :
+  ⊢ ⟨ ok ⟩ program x ⟨ var x --> 1 ⊕ Err ⟩.
 Proof.
   eapply RuleSeq.
   - eapply RulePlus.
     + eapply RuleCmd. eapply RuleAlloc.
     + eapply RuleCmd. eapply RuleAssign.
   - eapply RuleSplit; eauto using rules, rules_atom.
-    eapply RuleConsequence. 2: { eapply RuleCmd. eapply RuleStoreErr. }
+    eapply RuleConsequence.
     + apply null_implies_unmapped.
-    + intros ????. solve_eq_set.
+    + eapply RuleCmd. eapply RuleStoreErr.
+    + intros ????. simpgoal.
+Qed.
+
+(* Trace of program that leads to memory error, recovered from proof
+   using outcome logic *)
+Example error_witness x :
+  (program x , empty_state) ⇓ err.
+Proof.
+  edestruct (rules_sound _ _ _ (has_potential_memory_error x))
+    as [S [S' [H [_ Herr]]]].
+  - exists empty_state. split.
+    + eexists. eexists. reflexivity.
+    + apply eq_set_refl.
+  - specialize (H err) as [_ H].
+    destruct H as [σ [Heq Heval]].
+    + right. apply Herr. reflexivity.
+    + rewrite Heq in *. apply Heval.
 Qed.
