theories/assertion.v
@@ -1,0 +1,48 @@
+Require Import syntax.
+
+(* Atomic assertions (propositions) for 'ok' states *)
+Inductive okprop : Type :=
+| OkTrue
+| MapsTo (e : expr) (e : expr)
+| Mapped (e : expr)
+| Unmapped (e : expr)
+| Assigned (x : nat) (e : expr)
+.
+
+Notation "'ok'" := OkTrue (at level 55).
+Notation "e1 --> e2" := (MapsTo e1 e2) (at level 55).
+Notation "e --> -" := (Mapped e) (at level 55).
+Notation "e -/->" := (Unmapped e) (at level 55).
+Notation "x == e" := (Assigned x e) (at level 55).
+
+(* Atomic assertions (propositions) *)
+Inductive prop : Type :=
+| Ok : okprop -> prop
+| Err : prop
+.
+
+Notation "'error'" := Err.
+
+Coercion Ok : okprop >-> prop.
+
+(* Outcome logic assertion language *)
+Inductive assertion : Type :=
+| Top : assertion
+| Bot : assertion
+| Diverge : assertion
+| And : assertion -> assertion -> assertion
+| Or : assertion -> assertion -> assertion
+| Conj : assertion -> assertion -> assertion
+| Impl : assertion -> assertion -> assertion
+| Atomic : prop -> assertion
+.
+
+Coercion Atomic : prop >-> assertion.
+
+Notation "⊤" := Top.
+Notation "⊥" := Bot.
+Notation "⊤⊕" := Diverge.
+Notation "phi ∧ psi" := (And phi psi) (at level 70).
+Notation "phi ∨ psi" := (Or phi psi) (at level 70).
+Notation "phi ⊕ psi" := (Conj phi psi) (at level 80).
+Notation "phi ⇒ psi" := (Impl phi psi) (at level 60).
