theories/state.v
@@ -2,12 +2,37 @@ Require Import syntax.
 Require Import util.
 Require Import vec.
 
+(* Values that can be stored in the heap + stack: naturals or null *)
 Definition value := option nat.
 
+Definition is_true (v : value) : Prop :=
+  match v with
+  | Some n => n > 0
+  | None => False
+  end.
+
+Definition is_false (v : value) : Prop :=
+  match v with
+  | Some n => n = 0
+  | None => True
+  end.
+
+(* The local stack + associated operations/lemmas *)
 Definition stack := nat -> value.
-Definition heap := { n & vec n value }.
 
 Definition empty_stack : stack := fun _ => None.
+
+Definition insert (x : nat) (v : value) (s : stack) : stack :=
+  fun y => if Nat.eq_dec x y then v else s y.
+
+Lemma lookup_insert x v s : (insert x v s) x = v.
+Proof.
+  intros. unfold insert. destruct (Nat.eq_dec x x); congruence.
+Qed.
+
+(* The heap + associated operations/lemmas *)
+Definition heap := { n & vec n value }.
+
 Definition empty_heap : heap := existT _ O  tt.
 
 Definition newptr (h : heap) : heap * nat :=
@@ -31,6 +56,13 @@ Definition store (h : heap) (i : nat) (v : value) : heap :=
       existT _ n (update l i v)
   end.
 
+Definition mapsto (h : heap) (i : nat) (v : value) : Prop :=
+  match load h i with
+  | None => False
+  | Some v' => v = v'
+  end.
+
+(* A program state is either a stack and a heap or a memory error *)
 Definition state := ((stack * heap) + unit)%type.
 
 Definition good_state (s : stack) (h : heap) : state := inl (s , h).
@@ -42,40 +74,3 @@ Definition empty_state : state := <{ empty_stack, empty_heap }>.
 Definition mem_err : state := inr tt.
 
 Notation "'err'" := mem_err.
-
-Definition insert (x : nat) (v : value) (s : stack) : stack :=
-  fun y => if Nat.eq_dec x y then v else s y.
-
-Definition mapsto (h : heap) (i : nat) (v : value) : Prop :=
-  match load h i with
-  | None => False
-  | Some v' => v = v'
-  end.
-
-Definition is_true (v : value) : Prop :=
-  match v with
-  | Some n => n > 0
-  | None => False
-  end.
-
-Definition is_false (v : value) : Prop :=
-  match v with
-  | Some n => n = 0
-  | None => True
-  end.
-
-Lemma value_eq_dec (v1 v2 : value) : {v1 = v2} + {v1 <> v2}.
-Proof.
-  destruct v1 as [n1|]; destruct v2 as[n2|].
-  - destruct (Nat.eq_dec n1 n2).
-    + left. congruence.
-    + right. congruence.
-  - right. congruence.
-  - right. congruence.
-  - left. reflexivity.
-Qed.
-
-Lemma lookup_insert x v s : (insert x v s) x = v.
-Proof. 
-  intros. unfold insert. destruct (Nat.eq_dec x x); congruence.
-Qed.
