theories/theorems.v
@@ -1,0 +1,8 @@
+Require Import ol rules soundness.
+
+(* Any derivable OL triple is semantically valid (i.e. given the precondition,
+   any execution of the program results in the postcondition) *)
+Theorem rules_sound phi C psi :
+  ⊢ ⟨ phi ⟩ C ⟨ psi ⟩ ->
+  ⊨ ⟨ phi ⟩ C ⟨ psi ⟩.
+Proof. intros. induction H; eauto with sound_lemmas. Qed.
